Reimplement Matrix.Poly over array views

dist/Kuiper_ArrayView_Test1.cu
@@ -1,0 +1,24 @@
+
+
+#include "Kuiper_ArrayView_Test1.h"
+
+uint32_t Kuiper_ArrayView_Test1_test(uint32_t *a)
+{
+  return *a;
+}
+
+uint32_t Kuiper_ArrayView_Test1_test2(uint32_t *a)
+{
+  return a[49U];
+}
+
+void Kuiper_ArrayView_Test1_write1(uint32_t *a)
+{
+  *a = 123U;
+}
+
+void Kuiper_ArrayView_Test1_write2(uint32_t *a)
+{
+  a[49U] = 123U;
+}
+
